constr/destr int, simple, string; array in progress

src/cbor/CBOR.Steel.fst
@@ -21,6 +21,7 @@ type cbor_string = {
   typ: Cbor.major_type_byte_string_or_text_string;
   byte_length: U64.t;
   payload: LPS.byte_array;
+  footprint: LPA.array LPS.byte;
 }
 
 noeq
@@ -39,6 +40,7 @@ type cbor_tagged = {
 and cbor_array = {
   count: U64.t;
   payload: A.array cbor;
+  footprint: Ghost.erased (Seq.seq cbor);
 }
 
 and cbor_map_entry = {
@@ -59,6 +61,8 @@ and cbor =
 | CBOR_Case_Map of cbor_map
 | CBOR_Case_Simple_value of Cbor.simple_value
 | CBOR_Case_Serialized of cbor_serialized
+
+let dummy_cbor : cbor = CBOR_Case_Int64 ({ typ = Cbor.major_type_uint64; value = 0uL })
 
 let raw_data_item_match_serialized_prop
   (c: cbor)
@@ -126,6 +130,7 @@ let raw_data_item_match_string_prop
   | CBOR_Case_String c ->
     U64.v c.byte_length == LPA.length (LPA.array_of w) /\
     v == Cbor.String c.typ (LPA.contents_of w) /\
+    c.footprint == LPA.array_of w /\
     c.payload == a
   | _ -> False
 
@@ -165,11 +170,13 @@ let raw_data_item_match_tagged0
 let raw_data_item_match_array_prop
   (c: cbor)
   (v: Cbor.raw_data_item)
+  (s: Seq.seq cbor)
   (a: A.array cbor)
 : GTot prop
 = match c, v with
   | CBOR_Case_Array c, Cbor.Array l ->
     U64.v c.count == List.Tot.length l /\
+    Ghost.reveal c.footprint == s /\
     c.payload == a
   | _ -> False
 
@@ -183,7 +190,7 @@ let raw_data_item_match_array0
     A.pts_to a full_perm c' `star`
     raw_data_item_array_match c' (Cbor.Array?.v v) `star`
     pure (
-      raw_data_item_match_array_prop c v a
+      raw_data_item_match_array_prop c v c' a
     )
   ))
 
@@ -277,20 +284,20 @@ and raw_data_item_array_match0
   (v: list Cbor.raw_data_item)
 : Tot vprop
   (decreases v)
-= match v with
-  | [] -> raw_data_item_array_match_nil0 c
-  | _ :: _ -> raw_data_item_array_match_cons0 c v raw_data_item_match0 raw_data_item_array_match0
+= if Nil? v
+  then raw_data_item_array_match_nil0 c
+  else raw_data_item_array_match_cons0 c v raw_data_item_match0 raw_data_item_array_match0
 
 and raw_data_item_map_match0
   (c: Seq.seq cbor_map_entry)
   (v: list (Cbor.raw_data_item & Cbor.raw_data_item))
 : Tot vprop
   (decreases v)
-= match v with
-  | [] -> raw_data_item_map_match_nil0 c
-  | _ :: _ -> raw_data_item_map_match_cons0 c v raw_data_item_match0 raw_data_item_map_match0
+= if Nil? v
+  then raw_data_item_map_match_nil0 c
+  else raw_data_item_map_match_cons0 c v raw_data_item_match0 raw_data_item_map_match0
 
-irreducible
+// irreducible
 let raw_data_item_match : (phi: (
   (c: cbor) ->
   (v: Cbor.raw_data_item) ->
@@ -300,12 +307,310 @@ let raw_data_item_match : (phi: (
 
 let raw_data_item_match_eq : squash (raw_data_item_match == raw_data_item_match0) = ()
 
+let raw_data_item_array_match0_cons_eq
+  (c: Seq.seq cbor)
+  (v: list Cbor.raw_data_item)
+: Lemma
+  (requires (Cons? v))
+  (ensures (raw_data_item_array_match0 c v == raw_data_item_array_match_cons0 c v raw_data_item_match raw_data_item_array_match0))
+= let (a :: q) = v in
+  assert_norm (raw_data_item_array_match0 c (a :: q) == raw_data_item_array_match_cons0 c (a :: q) raw_data_item_match0 raw_data_item_array_match0)
+
 #set-options "--ide_id_info_off"
 
-let raw_data_item_match0_get_case
+irreducible
+let maybe_seq_cbor_uncons
+  (c: Seq.seq cbor)
+: Ghost (cbor & Seq.seq cbor)
+    (requires True)
+    (ensures (fun (hd, tl) ->
+      Seq.length c > 0 ==> c `Seq.equal` Seq.cons hd tl
+    ))
+= if Seq.length c = 0
+  then (dummy_cbor, c)
+  else (Seq.index c 0, Seq.slice c 1 (Seq.length c))
+
+let rewrite_with_implies
   (#opened: _)
+  (p q: vprop)
+: STGhost unit opened
+    p
+    (fun _ -> q `star` (q `implies_` p))
+    (p == q)
+    (fun _ -> True)
+= rewrite p q;
+  intro_implies q p emp (fun _ ->
+    rewrite q p
+  )
+
+#push-options "--z3rlimit 16"
+#restart-solver
+
+let list_cons_is_cons
+  (#t: Type)
+  (v: list t)
+  (a: t)
+  (q: list t)
+  (sq: squash (v == a :: q))
+: Tot (squash (Cons? v))
+= ()
+
+let raw_data_item_array_match0_cons_elim
+  (#opened: _)
+  (c: Seq.seq cbor)
+  (hd: cbor)
+  (tl: Seq.seq cbor)
+  (v: list Cbor.raw_data_item)
+  (a: Cbor.raw_data_item)
+  (q: list Cbor.raw_data_item)
+: STGhost unit opened
+    (raw_data_item_array_match0 c v)
+    (fun _ ->
+      raw_data_item_match hd a `star` raw_data_item_array_match0 tl q `star` (
+        (raw_data_item_match hd a `star` raw_data_item_array_match0 tl q) `implies_`
+        raw_data_item_array_match0 c v
+    ))
+    (v == a :: q /\
+      (Seq.length c > 0 ==> c `Seq.equal` Seq.cons hd tl)
+    )
+    (fun _ ->
+      c `Seq.equal` Seq.cons hd tl
+    )
+= let _v_cons : squash (Cons? v) = list_cons_is_cons v a q () in
+  raw_data_item_array_match0_cons_eq c v;
+  noop ();
+  rewrite_with_implies
+    (raw_data_item_array_match0 c v)
+    (raw_data_item_array_match_cons0 c v raw_data_item_match raw_data_item_array_match0);
+  let _ = gen_elim () in
+  let hd' = vpattern (fun hd -> raw_data_item_match hd _) in
+  let tl' = vpattern (fun tl -> raw_data_item_array_match0 tl _) in
+  Seq.lemma_cons_inj hd hd' tl tl';
+  noop ();
+  rewrite_with_implies
+    (raw_data_item_match _ (List.Tot.hd v))
+    (raw_data_item_match hd a);
+  rewrite_with_implies
+    (raw_data_item_array_match0 _ (List.Tot.tl v))
+    (raw_data_item_array_match0 tl q);
+  implies_join
+    (raw_data_item_match hd a)
+    (raw_data_item_match _ (List.Tot.hd v))
+    (raw_data_item_array_match0 tl q)    
+    (raw_data_item_array_match0 _ (List.Tot.tl v));
+  intro_implies
+    (raw_data_item_match hd a `star` raw_data_item_array_match0 tl q)
+    (raw_data_item_array_match_cons0 c v raw_data_item_match raw_data_item_array_match0)
+    ((raw_data_item_match hd a `star` raw_data_item_array_match0 tl q) `implies_`
+      (raw_data_item_match _ (List.Tot.hd v) `star` raw_data_item_array_match0 _ (List.Tot.tl v))
+    )
+    (fun _ ->
+      elim_implies
+        (raw_data_item_match hd a `star` raw_data_item_array_match0 tl q)
+        (raw_data_item_match _ (List.Tot.hd v) `star` raw_data_item_array_match0 _ (List.Tot.tl v));
+      noop ()
+    );
+  implies_trans
+    (raw_data_item_match hd a `star` raw_data_item_array_match0 tl q)
+    (raw_data_item_array_match_cons0 c v raw_data_item_match raw_data_item_array_match0)    
+    (raw_data_item_array_match0 c v)
+
+#pop-options
+
+let raw_data_item_array_match0_cons_intro
+  (#opened: _)
+  (c: Seq.seq cbor)
+  (hd: cbor)
+  (tl: Seq.seq cbor)
+  (v: list Cbor.raw_data_item)
+  (a: Cbor.raw_data_item)
+  (q: list Cbor.raw_data_item)
+: STGhost unit opened
+    (raw_data_item_match hd a `star` raw_data_item_array_match0 tl q)
+    (fun _ ->
+      raw_data_item_array_match0 c v `star`
+      (raw_data_item_array_match0 c v `implies_`
+        (raw_data_item_match hd a `star` raw_data_item_array_match0 tl q)
+      )
+    )
+    (v == a :: q /\
+      c `Seq.equal` Seq.cons hd tl
+    )
+    (fun _ -> True)
+= let _v_cons : squash (Cons? v) = list_cons_is_cons v a q () in
+  raw_data_item_array_match0_cons_eq c v;
+  noop ();
+  vpattern_rewrite (raw_data_item_match hd) (List.Tot.hd v);
+  vpattern_rewrite (raw_data_item_array_match0 tl) (List.Tot.tl v);
+  rewrite
+    (raw_data_item_array_match_cons0 c v raw_data_item_match raw_data_item_array_match0)
+    (raw_data_item_array_match0 c v);
+  intro_implies
+    (raw_data_item_array_match0 c v)
+    (raw_data_item_match hd a `star` raw_data_item_array_match0 tl q)
+    emp
+    (fun _ ->
+      raw_data_item_array_match0_cons_elim c hd tl v a q;
+      drop (
+        (raw_data_item_match hd a `star` raw_data_item_array_match0 tl q) `implies_`
+        (raw_data_item_array_match0 c v)
+      )
+    )
+
+let implies_emp_l
+  (#opened: _)
+  (p: vprop)
+: STGhostT unit opened
+    p
+    (fun _ -> emp `implies_` p)
+= intro_implies emp p p (fun _ -> noop ())
+
+let implies_with_tactic
+  (#opened: _)
+  (p q: vprop)
+: STGhost unit opened
+    emp
+    (fun _ -> p `implies_` q)
+    (requires FStar.Tactics.with_tactic init_resolve_tac (squash (p `equiv` q)))
+    (ensures fun _ -> True)
+= intro_implies p q emp (fun _ -> rewrite_equiv p q)
+
+let implies_concl_l
+  (#opened: _)
+  (p q r: vprop)
+: STGhostT unit opened
+    (p `star` (q `implies_` r))
+    (fun _ -> q `implies_` (p `star` r))
+= implies_with_tactic q (emp `star` q);
+  implies_emp_l p;
+  implies_join emp p q r;
+  implies_trans q (emp `star` q) (p `star` r)
+
+let implies_concl_r
+  (#opened: _)
+  (q r p: vprop)
+: STGhostT unit opened
+    (p `star` (q `implies_` r))
+    (fun _ -> q `implies_` (r `star` p))
+= implies_concl_l p q r;
+  implies_with_tactic (p `star` r) (r `star` p);
+  implies_trans q (p `star` r) (r `star` p)
+
+let implies_reg_l
+  (#opened: _)
+  (p q r: vprop)
+: STGhostT unit opened
+    (q `implies_` r)
+    (fun _ -> (p `star` q) `implies_` (p `star` r))
+= implies_with_tactic p p;
+  implies_join p p q r
+
+let implies_reg_r
+  (#opened: _)
+  (q r: vprop)
+  (p: vprop)
+: STGhostT unit opened
+    (q `implies_` r)
+    (fun _ -> (q `star` p) `implies_` (r `star` p))
+= implies_with_tactic p p;
+  implies_join q r p p
+
+let rec raw_data_item_array_match_append_strong
+  (#opened: _)
+  (c1 c2: Seq.seq cbor)
+  (v1 v2: list Cbor.raw_data_item)
+: STGhostT unit opened
+    (raw_data_item_array_match0 c1 v1 `star` raw_data_item_array_match0 c2 v2)
+    (fun _ -> raw_data_item_array_match0 (c1 `Seq.append` c2) (v1 `List.Tot.append` v2) `star`
+      (raw_data_item_array_match0 (c1 `Seq.append` c2) (v1 `List.Tot.append` v2) `implies_` (
+        raw_data_item_array_match0 c1 v1 `star` raw_data_item_array_match0 c2 v2
+    )))
+    (decreases v1)
+= match v1 with
+  | [] ->
+    Seq.append_empty_l c2;
+    rewrite_with_implies
+      (raw_data_item_array_match0 c1 v1)
+      (raw_data_item_array_match_nil0 c1);
+    let _ = gen_elim () in
+    rewrite_with_implies
+      (raw_data_item_array_match0 c2 v2)
+      (raw_data_item_array_match0 (c1 `Seq.append` c2) (v1 `List.Tot.append` v2));
+    elim_implies
+      (raw_data_item_array_match_nil0 c1)
+      (raw_data_item_array_match0 c1 v1);
+    implies_concl_l
+      (raw_data_item_array_match0 c1 v1)
+      (raw_data_item_array_match0 (c1 `Seq.append` c2) (v1 `List.Tot.append` v2))
+      (raw_data_item_array_match0 c2 v2)
+  | a1 :: v1' ->
+    let (b1, c1') = maybe_seq_cbor_uncons c1 in
+    noop ();
+    raw_data_item_array_match0_cons_elim
+      c1 b1 c1'
+      v1 a1 v1';
+    raw_data_item_array_match_append_strong c1' c2 v1' v2;
+    raw_data_item_array_match0_cons_intro
+      (c1 `Seq.append` c2) b1 (c1' `Seq.append` c2)
+      (v1 `List.Tot.append` v2) a1 (v1' `List.Tot.append` v2);
+    implies_reg_r
+      (raw_data_item_match b1 a1 `star` raw_data_item_array_match0 c1' v1')
+      (raw_data_item_array_match0 c1 v1)
+      (raw_data_item_array_match0 c2 v2);
+    implies_reg_l
+      (raw_data_item_match b1 a1)
+      (raw_data_item_array_match0 (c1' `Seq.append` c2) (v1' `List.Tot.append` v2))
+      (raw_data_item_array_match0 c1' v1' `star` raw_data_item_array_match0 c2 v2);
+    implies_with_tactic
+      (raw_data_item_match b1 a1 `star` (raw_data_item_array_match0 c1' v1' `star` raw_data_item_array_match0 c2 v2))
+      ((raw_data_item_match b1 a1 `star` raw_data_item_array_match0 c1' v1') `star` raw_data_item_array_match0 c2 v2);
+    implies_trans
+      (raw_data_item_array_match0 (c1 `Seq.append` c2) (v1 `List.Tot.append` v2))
+      (raw_data_item_match b1 a1 `star` raw_data_item_array_match0 (c1' `Seq.append` c2) (v1' `List.Tot.append` v2))
+      (raw_data_item_match b1 a1 `star` (raw_data_item_array_match0 c1' v1' `star` raw_data_item_array_match0 c2 v2));
+    implies_trans
+      (raw_data_item_array_match0 (c1 `Seq.append` c2) (v1 `List.Tot.append` v2))
+      (raw_data_item_match b1 a1 `star` (raw_data_item_array_match0 c1' v1' `star` raw_data_item_array_match0 c2 v2))
+      ((raw_data_item_match b1 a1 `star` raw_data_item_array_match0 c1' v1') `star` raw_data_item_array_match0 c2 v2);
+    implies_trans
+      (raw_data_item_array_match0 (c1 `Seq.append` c2) (v1 `List.Tot.append` v2))
+      ((raw_data_item_match b1 a1 `star` raw_data_item_array_match0 c1' v1') `star` raw_data_item_array_match0 c2 v2)
+      (raw_data_item_array_match0 c1 v1 `star` raw_data_item_array_match0 c2 v2)
+
+let raw_data_item_array_match0_singleton_intro
+  (#opened: _)
+  (c: Seq.seq cbor)
+  (b: cbor)
+  (v: list Cbor.raw_data_item)
+  (a: Cbor.raw_data_item)
+: STGhost unit opened
+    (raw_data_item_match b a)
+    (fun _ -> raw_data_item_array_match0 c v `star` (raw_data_item_array_match0 c v `implies_` raw_data_item_match b a))
+    (c `Seq.equal` Seq.create 1 b /\
+      v == [a]
+    )
+    (fun _ -> True)
+= noop ();
+  rewrite
+    (raw_data_item_array_match_nil0 Seq.empty)
+    (raw_data_item_array_match0 Seq.empty []);
+  raw_data_item_array_match0_cons_intro c b Seq.empty v a [];
+  intro_implies
+    (raw_data_item_match b a `star` raw_data_item_array_match0 Seq.empty [])
+    (raw_data_item_match b a)
+    emp
+    (fun _ ->
+      drop (raw_data_item_array_match0 Seq.empty [])
+    );
+  implies_trans
+    (raw_data_item_array_match0 c v)
+    (raw_data_item_match b a `star` raw_data_item_array_match0 Seq.empty [])
+    (raw_data_item_match b a)
+
+let raw_data_item_match_get_case
+  (#opened: _)
+  (#v: Cbor.raw_data_item)
   (c: cbor)
-  (v: Cbor.raw_data_item)
 : STGhost unit opened
     (raw_data_item_match c v)
     (fun _ -> raw_data_item_match c v)
@@ -335,18 +640,157 @@ let raw_data_item_match0_get_case
       let _ = gen_elim () in
       rewrite emp (raw_data_item_match c v)
 
-let rewrite_with_implies
+let raw_data_item_match_array_intro
   (#opened: _)
-  (p q: vprop)
-: STGhost unit opened
-    p
-    (fun _ -> q `star` (q `implies_` p))
-    (p == q)
-    (fun _ -> True)
-= rewrite p q;
-  intro_implies q p emp (fun _ ->
-    rewrite q p
-  )
+  (#c': Seq.seq cbor)
+  (#v': list Cbor.raw_data_item)
+  (a: A.array cbor)
+  (len: U64.t {
+    U64.v len == List.Tot.length v'
+  })
+: STGhostT unit opened
+    (A.pts_to a full_perm c' `star`
+      raw_data_item_array_match0 c' v')
+    (fun _ ->
+      raw_data_item_match
+        (CBOR_Case_Array ({
+          count = len;
+          payload = a;
+          footprint = c';
+        }))
+        (Cbor.Array v')
+    )
+= noop ();
+  rewrite_with_tactic
+    (raw_data_item_match_array0
+      (CBOR_Case_Array ({
+        count = len;
+        payload = a;
+        footprint = c';
+      }))
+      (Cbor.Array v')
+      raw_data_item_array_match0
+    )
+    (raw_data_item_match _ _)
+
+let raw_data_item_match_array_elim
+  (#opened: _)
+  (a: cbor_array)
+  (v: Cbor.raw_data_item)
+: STGhost (squash (Cbor.Array? v)) opened
+    (raw_data_item_match (CBOR_Case_Array a) v)
+    (fun _ ->
+      A.pts_to a.payload full_perm a.footprint `star`
+      raw_data_item_array_match0 a.footprint (Cbor.Array?.v v)
+    )
+    True
+    (fun _ -> U64.v a.count == List.Tot.length (Cbor.Array?.v v))
+= raw_data_item_match_get_case _;
+  let sq : squash (Cbor.Array? v) = () in
+  let Cbor.Array v' = v in
+  vpattern_rewrite (raw_data_item_match _) (Cbor.Array v');
+  rewrite_with_tactic
+    (raw_data_item_match _ _)
+    (raw_data_item_match_array0 (CBOR_Case_Array a) (Cbor.Array v') raw_data_item_array_match0);
+  let _ = gen_elim () in
+  rewrite (A.pts_to _ _ _) (A.pts_to a.payload full_perm a.footprint);
+  rewrite (raw_data_item_array_match0 _ _) (raw_data_item_array_match0 a.footprint (Cbor.Array?.v v));
+  sq
+
+let constr_cbor_array
+  (#c': Ghost.erased (Seq.seq cbor))
+  (#v': Ghost.erased (list Cbor.raw_data_item))
+  (a: A.array cbor)
+  (len: U64.t {
+    U64.v len == List.Tot.length v'
+  })
+: ST cbor
+    (A.pts_to a full_perm c' `star`
+      raw_data_item_array_match0 c' v')
+    (fun res ->
+      raw_data_item_match res (Cbor.Array v') `star`
+      (raw_data_item_match res (Cbor.Array v') `implies_`
+        (A.pts_to a full_perm c' `star`
+          raw_data_item_array_match0 c' v')
+      )
+    )
+    True
+    (fun res ->
+      res == CBOR_Case_Array ({
+        payload = a;
+        count = len;
+        footprint = c';
+      })
+    )
+= [@@inline_let]
+  let ares : cbor_array = {
+    count = len;
+    payload = a;
+    footprint = c';
+  }
+  in
+  [@@inline_let]
+  let res = CBOR_Case_Array ares in
+  raw_data_item_match_array_intro a len;
+  rewrite (raw_data_item_match _ _) (raw_data_item_match res (Cbor.Array v'));
+  intro_implies
+    (raw_data_item_match res (Cbor.Array v'))
+    (A.pts_to a full_perm c' `star`
+      raw_data_item_array_match0 c' v'
+    )
+    emp
+    (fun _ ->
+      rewrite (raw_data_item_match _ _) (raw_data_item_match (CBOR_Case_Array ares) (Cbor.Array v'));
+      let _ = raw_data_item_match_array_elim _ _ in
+      rewrite (A.pts_to _ _ _) (A.pts_to a full_perm c');
+      rewrite (raw_data_item_array_match0 _ _) (raw_data_item_array_match0 c' v')
+    );
+  return res
+
+[@@__reduce__]
+let maybe_cbor_array
+  (v: Cbor.raw_data_item)
+: GTot (list Cbor.raw_data_item)
+= match v with
+  | Cbor.Array l -> l
+  | _ -> []
+
+let destr_cbor_array
+  (#v: Ghost.erased Cbor.raw_data_item)
+  (a: cbor)
+: ST cbor_array
+    (raw_data_item_match a v)
+    (fun res ->
+      A.pts_to res.payload full_perm res.footprint `star`
+      raw_data_item_array_match0 res.footprint (maybe_cbor_array v) `star`
+      ((A.pts_to res.payload full_perm res.footprint `star`
+        raw_data_item_array_match0 res.footprint (maybe_cbor_array v)) `implies_`
+        raw_data_item_match a v
+      )
+    )
+    (CBOR_Case_Array? a)
+    (fun res ->
+      a == CBOR_Case_Array res /\
+      Cbor.Array? v /\
+      U64.v res.count == List.Tot.length (Cbor.Array?.v v)
+    )
+= raw_data_item_match_get_case _;
+  let CBOR_Case_Array res = a in
+  vpattern_rewrite
+    (fun a -> raw_data_item_match a _)
+    (CBOR_Case_Array res);
+  let _ = raw_data_item_match_array_elim _ _ in
+  vpattern_rewrite (raw_data_item_array_match0 _) (maybe_cbor_array v);
+  intro_implies
+    (A.pts_to res.payload full_perm res.footprint `star`
+      raw_data_item_array_match0 res.footprint (maybe_cbor_array v))
+    (raw_data_item_match a v)
+    emp
+    (fun _ ->
+      raw_data_item_match_array_intro _ res.count;
+      rewrite (raw_data_item_match _ _) (raw_data_item_match _ _)
+    );
+  return res
 
 let read_valid_cbor_from_buffer_with_size_strong
   (#va: LPS.v Cbor.parse_raw_data_item_kind Cbor.raw_data_item)
@@ -412,3 +856,569 @@ let read_valid_cbor_from_buffer
     )
 = let alen = LPS.get_parsed_size Cbor.jump_raw_data_item a in
   read_valid_cbor_from_buffer_with_size a alen
+
+let read_cbor_int64
+  (#va: Ghost.erased Cbor.raw_data_item)
+  (c: cbor)
+: ST cbor_int
+    (raw_data_item_match c (Ghost.reveal va))
+    (fun _ -> raw_data_item_match c (Ghost.reveal va))
+    (Cbor.Int64? (Ghost.reveal va))
+    (fun c' ->
+      Ghost.reveal va == Cbor.Int64 c'.typ c'.value
+    )
+= raw_data_item_match_get_case c;
+  match c with
+  | CBOR_Case_Int64 c' ->
+    rewrite_with_implies
+      (raw_data_item_match c (Ghost.reveal va))
+      (raw_data_item_match_int0 c (Ghost.reveal va));
+    let _ = gen_elim () in
+    elim_implies
+      (raw_data_item_match_int0 c (Ghost.reveal va))
+      (raw_data_item_match c (Ghost.reveal va));
+    return c'
+  | CBOR_Case_Serialized cs ->
+    rewrite_with_implies
+      (raw_data_item_match c (Ghost.reveal va))
+      (raw_data_item_match_serialized0 c (Ghost.reveal va));
+    let _ = gen_elim () in
+    vpattern_rewrite (fun a -> LPS.aparse Cbor.parse_raw_data_item a _) cs.payload;
+    let typ = Cbor.read_major_type cs.payload in
+    let value = Cbor.read_int64 cs.payload in
+    let c' : cbor_int = {
+      typ = typ;
+      value = value;
+    }
+    in
+    noop ();
+    elim_implies
+      (raw_data_item_match_serialized0 c (Ghost.reveal va))
+      (raw_data_item_match c (Ghost.reveal va));
+    return c'
+
+let destr_cbor_int64
+  (#va: Ghost.erased Cbor.raw_data_item)
+  (c: cbor)
+: ST cbor_int
+    (raw_data_item_match c (Ghost.reveal va))
+    (fun c' ->
+      raw_data_item_match (CBOR_Case_Int64 c') (Ghost.reveal va) `star`
+      (raw_data_item_match (CBOR_Case_Int64 c') (Ghost.reveal va) `implies_` raw_data_item_match c (Ghost.reveal va))
+    )
+    (Cbor.Int64? (Ghost.reveal va))
+    (fun c' ->
+      Ghost.reveal va == Cbor.Int64 c'.typ c'.value
+    )
+= let c' = read_cbor_int64 c in
+  rewrite
+    (raw_data_item_match_int0 (CBOR_Case_Int64 c') (Ghost.reveal va))
+    (raw_data_item_match (CBOR_Case_Int64 c') (Ghost.reveal va));
+  intro_implies
+    (raw_data_item_match (CBOR_Case_Int64 c') (Ghost.reveal va))
+    (raw_data_item_match c (Ghost.reveal va))
+    (raw_data_item_match c (Ghost.reveal va))
+    (fun _ -> drop (raw_data_item_match (CBOR_Case_Int64 c') (Ghost.reveal va)));
+  return c'
+
+let constr_cbor_int64
+  (ty: Cbor.major_type_uint64_or_neg_int64)
+  (value: U64.t)
+: ST cbor
+    emp
+    (fun c -> raw_data_item_match c (Cbor.Int64 ty value))
+    True
+    (fun c -> c == CBOR_Case_Int64 ({ typ = ty; value = value }))
+= [@@inline_let]
+  let c = CBOR_Case_Int64 ({ typ = ty; value = value }) in
+  noop ();
+  rewrite
+    (raw_data_item_match_int0 c (Cbor.Int64 ty value))
+    (raw_data_item_match c (Cbor.Int64 ty value));
+  return c
+
+let read_cbor_simple_value
+  (#va: Ghost.erased Cbor.raw_data_item)
+  (c: cbor)
+: ST Cbor.simple_value
+    (raw_data_item_match c (Ghost.reveal va))
+    (fun c' ->
+      raw_data_item_match c (Ghost.reveal va)
+    )
+    (Cbor.Simple? (Ghost.reveal va))
+    (fun c' -> Ghost.reveal va == Cbor.Simple c')
+= raw_data_item_match_get_case c;
+  match c with
+  | CBOR_Case_Simple_value c' ->
+    rewrite_with_implies
+      (raw_data_item_match c (Ghost.reveal va))
+      (raw_data_item_match_simple_value0 c (Ghost.reveal va));
+    let _ = gen_elim () in
+    elim_implies
+      (raw_data_item_match_simple_value0 c (Ghost.reveal va))
+      (raw_data_item_match c (Ghost.reveal va));
+    return c'
+  | CBOR_Case_Serialized cs ->
+    rewrite_with_implies
+      (raw_data_item_match c (Ghost.reveal va))
+      (raw_data_item_match_serialized0 c (Ghost.reveal va));
+    let _ = gen_elim () in
+    vpattern_rewrite (fun a -> LPS.aparse Cbor.parse_raw_data_item a _) cs.payload;
+    let c' = Cbor.read_simple_value cs.payload in
+    elim_implies
+      (raw_data_item_match_serialized0 c (Ghost.reveal va))
+      (raw_data_item_match c (Ghost.reveal va));
+    return c'
+
+let destr_cbor_simple_value
+  (#va: Ghost.erased Cbor.raw_data_item)
+  (c: cbor)
+: ST Cbor.simple_value
+    (raw_data_item_match c (Ghost.reveal va))
+    (fun c' ->
+      raw_data_item_match (CBOR_Case_Simple_value c') (Ghost.reveal va) `star`
+      (raw_data_item_match (CBOR_Case_Simple_value c') (Ghost.reveal va) `implies_` raw_data_item_match c (Ghost.reveal va))
+    )
+    (Cbor.Simple? (Ghost.reveal va))
+    (fun c' -> Ghost.reveal va == Cbor.Simple c')
+= let c' = read_cbor_simple_value c in
+  rewrite
+    (raw_data_item_match_simple_value0 (CBOR_Case_Simple_value c') (Ghost.reveal va))
+    (raw_data_item_match (CBOR_Case_Simple_value c') (Ghost.reveal va));
+  intro_implies
+    (raw_data_item_match (CBOR_Case_Simple_value c') (Ghost.reveal va))
+    (raw_data_item_match c (Ghost.reveal va))
+    (raw_data_item_match c (Ghost.reveal va))
+    (fun _ -> drop (raw_data_item_match (CBOR_Case_Simple_value c') (Ghost.reveal va)));
+  return c'
+
+let constr_cbor_simple_value
+  (value: Cbor.simple_value)
+: ST cbor
+    emp
+    (fun c -> raw_data_item_match c (Cbor.Simple value))
+    True
+    (fun c -> c == CBOR_Case_Simple_value value)
+= [@@inline_let]
+  let c = CBOR_Case_Simple_value value in
+  noop ();
+  rewrite
+    (raw_data_item_match_simple_value0 c (Cbor.Simple value))
+    (raw_data_item_match c (Cbor.Simple value));
+  return c
+
+let destr_cbor_string'
+  (#va: Ghost.erased Cbor.raw_data_item)
+  (c: cbor)
+: ST cbor_string
+    (raw_data_item_match c (Ghost.reveal va))
+    (fun c' ->
+      raw_data_item_match (CBOR_Case_String c') (Ghost.reveal va) `star`
+      (raw_data_item_match (CBOR_Case_String c') (Ghost.reveal va) `implies_` raw_data_item_match c (Ghost.reveal va))
+    )
+    (Cbor.String? (Ghost.reveal va))
+    (fun _ -> True)
+= raw_data_item_match_get_case c;
+  match c with
+  | CBOR_Case_String c' ->
+    rewrite_with_implies
+      (raw_data_item_match c (Ghost.reveal va))
+      (raw_data_item_match (CBOR_Case_String c') (Ghost.reveal va));
+    return c'
+  | CBOR_Case_Serialized cs ->
+    rewrite_with_implies
+      (raw_data_item_match c (Ghost.reveal va))
+      (raw_data_item_match_serialized0 c (Ghost.reveal va));
+    let _ = gen_elim () in
+    vpattern_rewrite (fun a -> LPS.aparse Cbor.parse_raw_data_item a _) cs.payload;
+    let va' = vpattern_replace (LPS.aparse Cbor.parse_raw_data_item _) in
+    let typ = Cbor.read_major_type cs.payload in
+    let len = Cbor.read_argument_as_uint64 cs.payload in
+    let payload = Cbor.focus_string cs.payload in
+    let _ = gen_elim () in
+    let vpl : LPA.v LPS.byte = vpattern_replace (fun vpl -> LPA.arrayptr payload vpl `star` (LPA.arrayptr payload vpl `implies_` LPS.aparse Cbor.parse_raw_data_item cs.payload va')) in
+    let c' : cbor_string = {
+      typ = typ;
+      byte_length = len;
+      payload = payload;
+      footprint = LPA.array_of vpl;
+    }
+    in
+    noop ();
+    intro_implies
+      (raw_data_item_match_string0 (CBOR_Case_String c') (Ghost.reveal va))
+      (raw_data_item_match_serialized0 c (Ghost.reveal va))
+      (LPA.arrayptr payload vpl `implies_` LPS.aparse Cbor.parse_raw_data_item cs.payload va')
+      (fun _ ->
+        let _ = gen_elim () in
+        rewrite (LPA.arrayptr _ _) (LPA.arrayptr payload vpl);
+        elim_implies
+          (LPA.arrayptr payload vpl)
+          (LPS.aparse Cbor.parse_raw_data_item cs.payload va');
+        noop ()
+      );
+    rewrite_with_implies
+      (raw_data_item_match_string0 (CBOR_Case_String c') (Ghost.reveal va))
+      (raw_data_item_match (CBOR_Case_String c') (Ghost.reveal va));
+    implies_trans
+      (raw_data_item_match (CBOR_Case_String c') (Ghost.reveal va))
+      (raw_data_item_match_string0 (CBOR_Case_String c') (Ghost.reveal va))
+      (raw_data_item_match_serialized0 c (Ghost.reveal va));
+    implies_trans
+      (raw_data_item_match (CBOR_Case_String c') (Ghost.reveal va))
+      (raw_data_item_match_serialized0 c (Ghost.reveal va))
+      (raw_data_item_match c (Ghost.reveal va));
+    return c'
+
+let destr_cbor_string
+  (#va: Ghost.erased Cbor.raw_data_item)
+  (c: cbor {Cbor.String? va})
+: STT cbor_string
+    (raw_data_item_match c (Ghost.reveal va))
+    (fun c' -> exists_ (fun vc' ->
+      LPA.arrayptr c'.payload vc' `star`
+      (LPA.arrayptr c'.payload vc' `implies_` raw_data_item_match c (Ghost.reveal va)) `star`
+      pure (
+        U64.v c'.byte_length == Seq.length (LPA.contents_of' vc') /\
+        Ghost.reveal va == Cbor.String c'.typ (LPA.contents_of vc')
+    )))
+= let c' = destr_cbor_string' c in
+  rewrite_with_implies
+    (raw_data_item_match (CBOR_Case_String c') (Ghost.reveal va))
+    (raw_data_item_match_string0 (CBOR_Case_String c') (Ghost.reveal va));
+  let _ = gen_elim () in
+  vpattern_rewrite (fun a -> LPA.arrayptr a _) c'.payload;
+  let vc' = vpattern_replace (LPA.arrayptr _) in
+  intro_implies
+    (LPA.arrayptr c'.payload vc')
+    (raw_data_item_match_string0 (CBOR_Case_String c') (Ghost.reveal va))
+    (pure (raw_data_item_match_string_prop (CBOR_Case_String c') (Ghost.reveal va) c'.payload vc')) // FIXME: WHY WHY WHY?
+    (fun _ ->
+      noop ()
+    );
+  implies_trans
+    (LPA.arrayptr c'.payload vc')
+    (raw_data_item_match_string0 (CBOR_Case_String c') (Ghost.reveal va))
+    (raw_data_item_match (CBOR_Case_String c') (Ghost.reveal va));
+  implies_trans
+    (LPA.arrayptr c'.payload vc')
+    (raw_data_item_match (CBOR_Case_String c') (Ghost.reveal va))
+    (raw_data_item_match c (Ghost.reveal va));
+  intro_exists vc' (fun vc' -> // FIXME: WHY WHY WHY?
+    LPA.arrayptr c'.payload vc' `star`
+      (LPA.arrayptr c'.payload vc' `implies_` raw_data_item_match c (Ghost.reveal va)) `star`
+      pure (
+        U64.v c'.byte_length == Seq.length (LPA.contents_of' vc') /\
+        Ghost.reveal va == Cbor.String c'.typ (LPA.contents_of vc')
+    )  
+  );
+  return c'
+
+let constr_cbor_string
+  (#va: LPA.v LPS.byte)
+  (typ: Cbor.major_type_byte_string_or_text_string)
+  (a: LPS.byte_array)
+  (len: U64.t {
+    U64.v len == Seq.length (LPA.contents_of va)
+  })
+: STT cbor
+    (LPA.arrayptr a va)
+    (fun c' ->
+      raw_data_item_match c' (Cbor.String typ (LPA.contents_of va)) `star`
+      (raw_data_item_match c' (Cbor.String typ (LPA.contents_of va)) `implies_`
+        LPA.arrayptr a va
+      )
+    )
+= [@@inline_let]
+  let c' = CBOR_Case_String ({
+    typ = typ;
+    payload = a;
+    byte_length = len;
+    footprint = LPA.array_of va;
+  })
+  in
+  noop ();
+  rewrite_with_implies
+    (raw_data_item_match_string0 c' (Cbor.String typ (LPA.contents_of va)))
+    (raw_data_item_match c' (Cbor.String typ (LPA.contents_of va)));
+  intro_implies
+    (raw_data_item_match_string0 c' (Cbor.String typ (LPA.contents_of va)))
+    (LPA.arrayptr a va)
+    emp
+    (fun _ ->
+      let _ = gen_elim () in
+      rewrite (LPA.arrayptr _ _) (LPA.arrayptr a va)
+    );
+  implies_trans
+    (raw_data_item_match c' (Cbor.String typ (LPA.contents_of va)))
+    (raw_data_item_match_string0 c' (Cbor.String typ (LPA.contents_of va)))
+    (LPA.arrayptr a va);
+  return c'
+
+let read_cbor_array_payload_invariant
+  (vl0: LPS.v LowParse.Spec.List.parse_list_kind (list Cbor.raw_data_item))
+  (l0: LPS.byte_array)
+  (a0: A.array cbor)
+  (pn: R.ref U64.t)
+  (pa2: R.ref (A.array cbor))
+  (pr: R.ref LPS.byte_array)
+: Tot vprop
+= exists_ (fun a1 -> exists_ (fun a2 -> exists_ (fun s1 -> exists_ (fun s2 -> exists_ (fun l1 -> exists_ (fun r -> exists_ (fun vr -> exists_ (fun n ->
+    A.pts_to a1 full_perm s1 `star`
+    R.pts_to pa2 full_perm a2 `star`
+    A.pts_to a2 full_perm s2 `star`
+    raw_data_item_array_match0 s1 l1 `star`
+    R.pts_to pr full_perm r `star`
+    LPS.aparse (LowParse.Spec.List.parse_list Cbor.parse_raw_data_item) r vr `star`
+    ((raw_data_item_array_match0 s1 l1 `star` LPS.aparse (LowParse.Spec.List.parse_list Cbor.parse_raw_data_item) r vr) `implies_`
+      LPS.aparse (LowParse.Spec.List.parse_list Cbor.parse_raw_data_item) l0 vl0) `star`
+    R.pts_to pn full_perm n `star`
+    pure (
+      A.adjacent a1 a2 /\
+      A.merge_into a1 a2 a0 /\
+      U64.v n == List.Tot.length vr.LPS.contents /\
+      U64.v n == Seq.length s2 /\
+      List.Tot.append l1 vr.LPS.contents == vl0.LPS.contents
+  )))))))))
+
+assume val read_cbor_array_payload
+  (n0: U64.t)
+  (vl0: LPS.v (LowParse.Spec.VCList.parse_nlist_kind (U64.v n0) Cbor.parse_raw_data_item_kind) (LowParse.Spec.VCList.nlist (U64.v n0) Cbor.raw_data_item))
+  (l0: LPS.byte_array)
+  (#va0: Ghost.erased (Seq.seq cbor))
+  (a0: A.array cbor)
+: STT (Ghost.erased (Seq.seq cbor))
+    (A.pts_to a0 full_perm va0 `star`
+      LPS.aparse (LowParse.Spec.VCList.parse_nlist (U64.v n0) Cbor.parse_raw_data_item) l0 vl0
+    )
+    (fun res ->
+      A.pts_to a0 full_perm res `star`
+      raw_data_item_array_match0 res vl0.contents `star`
+      (raw_data_item_array_match0 res vl0.contents `implies_`
+        LPS.aparse (LowParse.Spec.VCList.parse_nlist (U64.v n0) Cbor.parse_raw_data_item) l0 vl0
+      )
+    )
+
+let rewrite_aparse_with_implies
+  (#opened: _)
+  (#k1: LPS.parser_kind)
+  (#t1: Type)
+  (#p1: LPS.parser k1 t1)
+  (#y1: LPS.v k1 t1)
+  (a: LPS.byte_array)
+  (#k2: LPS.parser_kind)
+  (#t2: Type)
+  (p2: LPS.parser k2 t2)
+: STGhost (LPS.v k2 t2) opened
+    (LPS.aparse p1 a y1)
+    (fun y2 -> LPS.aparse p2 a y2 `star` (LPS.aparse p2 a y2 `implies_` LPS.aparse p1 a y1))
+    (t1 == t2 /\ (forall bytes . LPS.parse p1 bytes == LPS.parse p2 bytes))
+    (fun y2 ->
+      t1 == t2 /\
+      LPS.array_of' y1 == LPS.array_of' y2 /\
+      y1.contents == y2.contents
+    )
+= let y2 = LPS.rewrite_aparse a p2 in
+  intro_implies
+    (LPS.aparse p2 a y2)
+    (LPS.aparse p1 a y1)
+    emp
+    (fun _ ->
+      let _ = LPS.rewrite_aparse a p1 in
+      vpattern_rewrite (LPS.aparse _ a) y1
+    );
+  y2
+
+let vpattern_rewrite_with_implies
+  (#opened: _)
+  (#a: Type)
+  (#x1: a)
+  (p: a -> vprop)
+  (x2: a)
+: STGhost unit opened
+    (p x1)
+    (fun _ -> p x2 `star` (p x2 `implies_` p x1))
+    (x1 == x2)
+    (fun _ -> True)
+= rewrite_with_implies (p x1) (p x2)
+
+[@@__reduce__]
+let read_cbor_array_post_success
+  (c: cbor_array)
+: Tot vprop
+= exists_ (A.pts_to c.payload full_perm) `star`
+  pure (
+    A.is_full_array c.payload
+  )
+
+let read_cbor_array_post
+  (input: cbor)
+  (res: cbor)
+: Tot vprop
+= if CBOR_Case_Serialized? input && CBOR_Case_Array? res
+  then read_cbor_array_post_success (CBOR_Case_Array?._0 res)
+  else emp
+
+inline_for_extraction
+noextract
+let read_cbor_array_noop
+  (#obj: Ghost.erased Cbor.raw_data_item)
+  (input: cbor)
+: STT cbor
+    (raw_data_item_match input obj)
+    (fun res ->
+      raw_data_item_match res obj `star`
+      (raw_data_item_match res obj `implies_`
+        (raw_data_item_match input obj `star` read_cbor_array_post input res)
+      )
+    )
+= implies_with_tactic (raw_data_item_match input obj) (raw_data_item_match input obj);
+  rewrite emp (read_cbor_array_post input input);
+  implies_concl_r (raw_data_item_match input obj) (raw_data_item_match input obj) (read_cbor_array_post input input);
+  return input
+
+let array_pts_to_or_null
+  (#t: Type)
+  (a: A.array t)
+  (v: Seq.seq t)
+: Tot vprop
+= if A.is_null a
+  then emp
+  else A.pts_to a full_perm v
+
+inline_for_extraction
+noextract
+let array_alloc
+  (#t: Type)
+  (init: t)
+  (n: SZ.t)
+: ST (A.array t)
+    emp
+    (fun res -> array_pts_to_or_null res (Seq.create (SZ.v n) init))
+    True
+    (fun res ->
+      if A.is_null res
+      then True
+      else A.length res == SZ.v n /\ A.is_full_array res
+    )
+= let res = A.alloc init n in
+  A.pts_to_not_null res _;
+  rewrite
+    (A.pts_to res full_perm (Seq.create (SZ.v n) init))
+    (array_pts_to_or_null res (Seq.create (SZ.v n) init));
+  return res
+
+let read_cbor_array
+  (#obj: Ghost.erased Cbor.raw_data_item)
+  (input: cbor)
+: ST cbor
+    (raw_data_item_match input obj)
+    (fun res ->
+      raw_data_item_match res obj `star`
+      (raw_data_item_match res obj `implies_`
+        (raw_data_item_match input obj `star` read_cbor_array_post input res)
+      )
+    )
+    (Cbor.Array? obj)
+    (fun _ -> True)
+= raw_data_item_match_get_case input;
+  match input with
+  | CBOR_Case_Array _ -> read_cbor_array_noop input
+  | CBOR_Case_Serialized s ->
+      rewrite_with_implies
+        (raw_data_item_match input obj)
+        (raw_data_item_match_serialized0 input obj);
+      let _ = gen_elim () in
+      vpattern_rewrite_with_implies
+        (fun a -> LPS.aparse Cbor.parse_raw_data_item a _)
+        s.payload;
+      intro_implies
+        (LPS.aparse Cbor.parse_raw_data_item s.payload _)
+        (raw_data_item_match_serialized0 input obj)
+        (LPS.aparse Cbor.parse_raw_data_item s.payload _ `implies_`
+          LPS.aparse Cbor.parse_raw_data_item _ _
+        )
+        (fun _ ->
+          elim_implies
+            (LPS.aparse Cbor.parse_raw_data_item s.payload _)
+            (LPS.aparse Cbor.parse_raw_data_item _ _);
+          noop ()
+        );
+      implies_trans
+        (LPS.aparse Cbor.parse_raw_data_item s.payload _)
+        (raw_data_item_match_serialized0 input obj)
+        (raw_data_item_match input obj);
+      R.with_local 0uL (fun plen ->
+      R.with_local s.payload (fun pa ->
+        let w = CBOR.SteelST.Array.focus_array plen pa s.payload in
+        implies_trans
+          (LPS.aparse (LowParse.Spec.VCList.parse_nlist (U64.v w.n) Cbor.parse_raw_data_item) w.a _)
+          (LPS.aparse Cbor.parse_raw_data_item s.payload _)
+          (raw_data_item_match input obj);
+        let len = R.read plen in
+        let _ = A.intro_fits_u64 () in
+        let a0 = array_alloc dummy_cbor (SZ.uint64_to_sizet len) in
+        if (A.is_null a0)
+        then begin
+          noop ();
+          rewrite
+            (array_pts_to_or_null a0 _)
+            emp;
+          elim_implies
+            (LPS.aparse (LowParse.Spec.VCList.parse_nlist (U64.v w.n) Cbor.parse_raw_data_item) w.a _)
+            (raw_data_item_match input obj);
+          let res = read_cbor_array_noop input in
+          return res
+        end else begin
+          noop ();
+          rewrite
+            (array_pts_to_or_null a0 _)
+            (A.pts_to a0 full_perm (Seq.create (U64.v len) dummy_cbor));
+          let vl = rewrite_aparse_with_implies
+            w.a
+            (LowParse.Spec.VCList.parse_nlist (U64.v len) Cbor.parse_raw_data_item)
+          in
+          let a = R.read pa in
+          vpattern_rewrite_with_implies
+            (fun a -> LPS.aparse (LowParse.Spec.VCList.parse_nlist (U64.v len) Cbor.parse_raw_data_item) a _)
+            a;
+          implies_trans
+            (LPS.aparse (LowParse.Spec.VCList.parse_nlist (U64.v len) Cbor.parse_raw_data_item) a _)
+            (LPS.aparse (LowParse.Spec.VCList.parse_nlist (U64.v len) Cbor.parse_raw_data_item) _ _)
+            (LPS.aparse (LowParse.Spec.VCList.parse_nlist (U64.v w.n) Cbor.parse_raw_data_item) _ _);
+          implies_trans
+            (LPS.aparse (LowParse.Spec.VCList.parse_nlist (U64.v len) Cbor.parse_raw_data_item) a _)
+            (LPS.aparse (LowParse.Spec.VCList.parse_nlist (U64.v w.n) Cbor.parse_raw_data_item) _ _)
+            (raw_data_item_match input obj);
+          let va = read_cbor_array_payload len vl a a0 in
+          implies_trans
+            (raw_data_item_array_match0 va vl.contents)
+            (LPS.aparse (LowParse.Spec.VCList.parse_nlist (U64.v len) Cbor.parse_raw_data_item) a _)
+            (raw_data_item_match input obj);
+          let res = constr_cbor_array a0 len in
+          vpattern_rewrite
+            (fun ar -> raw_data_item_match _ ar `star` (raw_data_item_match _ ar `implies_` (A.pts_to _ _ _ `star` raw_data_item_array_match0 _ _)))
+            obj;
+          intro_implies
+            (A.pts_to a0 full_perm va `star` raw_data_item_array_match0 va vl.contents)
+            (raw_data_item_array_match0 va vl.contents `star` read_cbor_array_post input res)
+            emp
+            (fun _ ->
+              vpattern_rewrite (fun a0 -> A.pts_to a0 _ _) (CBOR_Case_Array?._0 res).payload;
+              rewrite (read_cbor_array_post_success (CBOR_Case_Array?._0 res)) (read_cbor_array_post input res)
+            );
+          implies_reg_r
+            (raw_data_item_array_match0 va vl.contents)
+            (raw_data_item_match input obj)
+            (read_cbor_array_post input res);
+          implies_trans
+            (raw_data_item_match res obj)
+            (A.pts_to a0 full_perm va `star` raw_data_item_array_match0 va vl.contents)
+            (raw_data_item_array_match0 va vl.contents `star` read_cbor_array_post input res);
+          implies_trans
+            (raw_data_item_match res obj)
+            (raw_data_item_array_match0 va vl.contents `star` read_cbor_array_post input res)
+            (raw_data_item_match input obj `star` read_cbor_array_post input res);
+          return res
+        end
+      ))
